lib/sep_algebra/Sep_Cancel.thy
@@ -16,59 +16,53 @@ begin
 
 
 lemma sep_curry': "\<lbrakk>(P \<and>* F) s; \<And>s. (Q \<and>* P \<and>* F) s \<Longrightarrow> R s\<rbrakk> \<Longrightarrow> (Q \<longrightarrow>* R) s"
-by (metis (full_types) sep.mult_commute sep_curry)
+  by (metis (full_types) sep.mult_commute sep_curry)
 
-lemma sep_conj_sep_impl_safe:  "(P \<longrightarrow>* P') s \<Longrightarrow> (\<And>s. ((P \<longrightarrow>* P') \<and>* Q) s \<Longrightarrow> (Q') s) \<Longrightarrow> (Q \<longrightarrow>* Q') s" 
- apply (erule sep_curry[rotated])
- apply (clarsimp)
-done
+lemma sep_conj_sep_impl_safe: 
+  "(P \<longrightarrow>* P') s \<Longrightarrow> (\<And>s. ((P \<longrightarrow>* P') \<and>* Q) s \<Longrightarrow> (Q') s) \<Longrightarrow> (Q \<longrightarrow>* Q') s" 
+  by (rule sep_curry)
 
 lemma  sep_conj_sep_impl_safe': "P s \<Longrightarrow> (\<And>s. (P \<and>* Q) s \<Longrightarrow> (P \<and>* R) s) \<Longrightarrow> (Q \<longrightarrow>* P \<and>* R) s" 
- apply (erule sep_curry[rotated])
- apply (clarsimp)
-done
+  by (rule sep_curry)
 
 lemma sep_wand_lens_simple: "(\<And>s. T s = (Q \<and>* R) s) \<Longrightarrow> (P \<longrightarrow>* T) s \<Longrightarrow> (P \<longrightarrow>* Q \<and>* R) s"
-   apply (clarsimp simp: sep_impl_def)
-done
-
+  by (clarsimp simp: sep_impl_def)
 
 schematic_goal schem_impAny: " (?C \<and>* B) s \<Longrightarrow> A s" by (erule sep_mp)
 
 ML {* 
-
-   fun sep_cancel_tactic ctxt concl  = 
-       let val thms = rev (SepCancel_Rules.get ctxt)
-           val tac  =  assume_tac ctxt ORELSE'
-                       eresolve_tac ctxt [@{thm sep_mp}, @{thm sep_conj_empty}, @{thm sep_empty_conj}]
-                       ORELSE' sep_erule_tactic ctxt thms
-           val direct_tac = eresolve_tac ctxt thms
-           val safe_sep_wand_tac = rotator' ctxt (resolve0_tac [@{thm sep_wand_lens_simple}]) (eresolve0_tac [@{thm sep_conj_sep_impl_safe'}])
-           fun sep_cancel_tactic_inner true   = sep_erule_full_tac' tac ctxt |
-               sep_cancel_tactic_inner false  = sep_erule_full_tac tac ctxt               
-   in sep_cancel_tactic_inner concl ORELSE'
+  fun sep_cancel_tactic ctxt concl  = 
+    let val thms = rev (SepCancel_Rules.get ctxt)
+        val tac  = assume_tac ctxt ORELSE'
+                   eresolve_tac ctxt [@{thm sep_mp}, @{thm sep_conj_empty}, @{thm sep_empty_conj}] ORELSE'
+                   sep_erule_tactic ctxt thms
+        val direct_tac = eresolve_tac ctxt thms
+        val safe_sep_wand_tac = rotator' ctxt (resolve0_tac [@{thm sep_wand_lens_simple}]) (eresolve0_tac [@{thm sep_conj_sep_impl_safe'}])
+        fun sep_cancel_tactic_inner true   = sep_erule_full_tac' tac ctxt
+          | sep_cancel_tactic_inner false  = sep_erule_full_tac tac ctxt
+  in sep_cancel_tactic_inner concl ORELSE'
       eresolve_tac ctxt [@{thm sep_curry'}, @{thm sep_conj_sep_impl_safe}, @{thm sep_imp_empty}, @{thm sep_empty_imp'}] ORELSE'
       safe_sep_wand_tac ORELSE'
       direct_tac
-   end;
+  end
 
+  fun sep_cancel_tactic' ctxt concl =
+    let
+      val sep_cancel = sep_cancel_tactic ctxt
+    in 
+      (sep_flatten ctxt THEN_ALL_NEW sep_cancel concl) ORELSE' sep_cancel concl
+    end
 
-   fun sep_cancel_tactic' ctxt concl =
-       let val sep_cancel =  (sep_cancel_tactic ctxt)
-    in ((sep_flatten ctxt) THEN_ALL_NEW sep_cancel concl) ORELSE' sep_cancel concl
- end;
-
-   fun sep_cancel_method (concl,_) ctxt = SIMPLE_METHOD' (sep_cancel_tactic' ctxt concl)
+  fun sep_cancel_method (concl,_) ctxt = SIMPLE_METHOD' (sep_cancel_tactic' ctxt concl)
   
-  val sep_cancel_syntax = Method.sections [
-    Args.add -- Args.colon >> K (Method.modifier SepCancel_Rules.add @{here})];
+  val sep_cancel_syntax =
+    Method.sections [Args.add -- Args.colon >> K (Method.modifier SepCancel_Rules.add @{here})];
   
-  val sep_cancel_syntax' = (Scan.lift (Args.mode "concl") -- sep_cancel_syntax)
-  
+  val sep_cancel_syntax' =
+    Scan.lift (Args.mode "concl") -- sep_cancel_syntax  
 *}
 
-method_setup sep_cancel = {*
-    sep_cancel_syntax'  >> (sep_cancel_method)
-*}{* Simple elimination of conjuncts *}
+method_setup sep_cancel = 
+  {* sep_cancel_syntax' >> sep_cancel_method *}  {* Simple elimination of conjuncts *}
 
 end
