lib/sep_algebra/Sep_Select.thy
@@ -15,37 +15,38 @@ begin
 ML_file "sep_tactics.ML"
 
 ML{* 
- structure SepSelect_Rules = Named_Thms (
-  val name = @{binding "sep_select"};
-  val description = "sep_select rules";
-  );
+  structure SepSelect_Rules = Named_Thms (
+    val name = @{binding "sep_select"}
+    val description = "sep_select rules"
+  )
 *}
 setup SepSelect_Rules.setup
 
 ML {*
   structure SepSelectAsm_Rules = Named_Thms (
-    val name = @{binding "sep_select_asm"};
-    val description = "sep_select_asm rules";
-  );
+    val name = @{binding "sep_select_asm"}
+    val description = "sep_select_asm rules"
+  )
 *}
-
 setup SepSelectAsm_Rules.setup
 
 ML {*
   fun sep_selects_tactic ns ctxt =
-      let val thms = SepSelect_Rules.get ctxt in
-      sep_select_tactic (resolve_tac ctxt thms) ns ctxt  
-  end;
+  let
+    val thms = SepSelect_Rules.get ctxt
+  in
+    sep_select_tactic (resolve_tac ctxt thms) ns ctxt
+  end
   
   fun sep_select_asms_tactic ns ctxt =
-      let val thms = SepSelectAsm_Rules.get ctxt in
-      sep_select_tactic (dresolve_tac ctxt thms) ns ctxt  
-  end; 
+  let
+    val thms = SepSelectAsm_Rules.get ctxt
+  in
+    sep_select_tactic (dresolve_tac ctxt thms) ns ctxt
+  end
 
-  fun sep_select_asms_method ns ctxt = SIMPLE_METHOD' 
-                                       (sep_select_asms_tactic ns ctxt)
-  fun sep_selects_method ns ctxt     = SIMPLE_METHOD' 
-                                       (sep_selects_tactic ns ctxt)
+  fun sep_select_asms_method ns ctxt = SIMPLE_METHOD' (sep_select_asms_tactic ns ctxt)
+  fun sep_selects_method ns ctxt     = SIMPLE_METHOD' (sep_selects_tactic ns ctxt)
 *}
 
 lemma sep_eq: "(\<And>s. T s = (P \<and>* R) s) \<Longrightarrow> T s \<Longrightarrow> (P \<and>* R) s" by clarsimp
@@ -64,18 +65,19 @@ method_setup sep_select = {*
 
 
 ML {* 
- fun sep_select_generic_method_inner ((lens, n), asm) ctxt =
-   let val lens_tac = (if asm then (dresolve_tac ctxt lens) else (resolve_tac ctxt lens))
-    in sep_select_method lens_tac n ctxt
-  end;
+  fun sep_select_generic_method_inner ((lens, n), asm) ctxt =
+  let
+    val lens_tac = if asm then dresolve_tac ctxt lens else resolve_tac ctxt lens
+  in
+    sep_select_method lens_tac n ctxt
+  end
 
-  fun sep_select_generic_method asm thms ns ctxt =
-      sep_select_generic_method_inner ((thms,ns),asm) ctxt
+  fun sep_select_generic_method asm thms ns = sep_select_generic_method_inner ((thms,ns),asm)
 *}
 
 method_setup sep_select_gen = {*
- Attrib.thms --| (Scan.lift Args.colon) -- Scan.lift (Scan.repeat Parse.int) -- (Scan.lift (Args.mode "asm")) >>
- sep_select_generic_method_inner
+  Attrib.thms --| Scan.lift Args.colon -- Scan.lift (Scan.repeat Parse.int) -- Scan.lift (Args.mode "asm") >>
+  sep_select_generic_method_inner
 *}
 
 end
