lib/sep_algebra/Sep_Tactic_Helpers.thy
@@ -15,34 +15,31 @@ begin
 lemmas sep_curry = sep_conj_sep_impl[rotated] 
 
 lemma sep_mp: "((Q \<longrightarrow>* R) \<and>* Q) s \<Longrightarrow> R s"
-  by (clarsimp simp: sep_conj_def sep_impl_def)
+  by (rule sep_conj_sep_impl2)
 
 lemma sep_mp_frame: "((Q \<longrightarrow>* R) \<and>* Q \<and>* R') s \<Longrightarrow> (R \<and>* R') s"
-    apply (clarsimp simp: sep_conj_assoc[symmetric])
-    apply (erule sep_conj_impl)
-    apply (erule sep_mp)
-    apply (assumption)
-done
+  apply (clarsimp simp: sep_conj_assoc[symmetric])
+  apply (erule sep_conj_impl)
+   apply (erule (1) sep_mp)
+  done
 
 lemma sep_empty_conj: "P s \<Longrightarrow> (\<box> \<and>* P) s"
-  apply (clarsimp)
-done
+  by clarsimp
 
 lemma sep_conj_empty: "(\<box> \<and>* P)  s \<Longrightarrow> P s"
-  apply (clarsimp)
-done
+  by clarsimp
 
 lemma sep_empty_imp: "(\<box> \<longrightarrow>* P) s \<Longrightarrow> P s"
   apply (clarsimp simp: sep_impl_def)
   apply (erule_tac x=0 in allE)
   apply (clarsimp)
-done
+  done
 
 lemma sep_empty_imp': "(\<box> \<longrightarrow>* P) s \<Longrightarrow> (\<And>s. P s \<Longrightarrow> Q s) \<Longrightarrow> Q s"
   apply (clarsimp simp: sep_impl_def)
   apply (erule_tac x=0 in allE)
   apply (clarsimp)
-done
+  done
 
 lemma sep_imp_empty: " P s \<Longrightarrow> (\<And>s. P s \<Longrightarrow> Q s) \<Longrightarrow> (\<box> \<longrightarrow>* Q) s"
   by (erule sep_conj_sep_impl, clarsimp)
